CLean.lean
@@ -5,4 +5,5 @@ import CLean.Typing
 import CLean.Helpers
 import CLean.Semantics
 import CLean.Lemmas
+import CLean.Execution
 import CLean.Examples
